SimGlobal with no index

ems/SimGlobal2.v
@@ -86,68 +86,70 @@ Inductive _simg
     _simg simg RR f_src f_tgt itr_src itr_tgt
 .
 
-Lemma _simg_ind2 (r P: forall R0 R1 (RR: R0 -> R1 -> Prop), bool -> bool -> (itree eventE R0) -> (itree eventE R1) -> Prop)
+Lemma _simg_ind2 (r: forall R0 R1 (RR: R0 -> R1 -> Prop), bool -> bool -> (itree eventE R0) -> (itree eventE R1) -> Prop)
+      R0 R1 (RR: R0 -> R1 -> Prop)
+      (P: bool -> bool -> (itree eventE R0) -> (itree eventE R1) -> Prop)
       (RET: forall
-          R0 R1 (RR: R0 -> R1 -> Prop) f_src f_tgt
+          f_src f_tgt
           r_src r_tgt
           (SIM: RR r_src r_tgt),
-          P _ _ RR f_src f_tgt (Ret r_src) (Ret r_tgt))
+          P f_src f_tgt (Ret r_src) (Ret r_tgt))
       (SYSCALL: forall
-          R0 R1 (RR: R0 -> R1 -> Prop) f_src f_tgt
+          f_src f_tgt
           ktr_src0 ktr_tgt0 fn varg rvs
           (SIM: forall x_src x_tgt (EQ: x_src = x_tgt), r _ _ RR true true (ktr_src0 x_src) (ktr_tgt0 x_tgt)),
-          P _ _ RR f_src f_tgt (trigger (Syscall fn varg rvs) >>= ktr_src0) (trigger (Syscall fn varg rvs) >>= ktr_tgt0))
+          P f_src f_tgt (trigger (Syscall fn varg rvs) >>= ktr_src0) (trigger (Syscall fn varg rvs) >>= ktr_tgt0))
       (TAUL: forall
-          R0 R1 (RR: R0 -> R1 -> Prop) f_src f_tgt
+          f_src f_tgt
           itr_src0 itr_tgt0
           (TAUL: True)
           (SIM: _simg r RR true f_tgt itr_src0 itr_tgt0)
-          (IH: P _ _ RR true f_tgt itr_src0 itr_tgt0),
-          P _ _ RR f_src f_tgt (tau;; itr_src0) (itr_tgt0))
+          (IH: P true f_tgt itr_src0 itr_tgt0),
+          P f_src f_tgt (tau;; itr_src0) (itr_tgt0))
       (TAUR: forall
-          R0 R1 (RR: R0 -> R1 -> Prop) f_src f_tgt
+          f_src f_tgt
           itr_src0 itr_tgt0
           (TAUR: True)
           (SIM: _simg r RR f_src true itr_src0 itr_tgt0)
-          (IH: P _ _ RR f_src true itr_src0 itr_tgt0),
-          P _ _ RR f_src f_tgt (itr_src0) (tau;;itr_tgt0))
+          (IH: P f_src true itr_src0 itr_tgt0),
+          P f_src f_tgt (itr_src0) (tau;;itr_tgt0))
       (CHOOSEL: forall
-          R0 R1 (RR: R0 -> R1 -> Prop) f_src f_tgt
+          f_src f_tgt
           X ktr_src0 itr_tgt0
           (CHOOSEL: True)
-          (SIM: exists x, <<SIM: _simg r RR true f_tgt (ktr_src0 x) itr_tgt0>> /\ <<IH: P _ _ RR true f_tgt (ktr_src0 x) itr_tgt0>>),
-          P _ _ RR f_src f_tgt (trigger (Choose X) >>= ktr_src0) (itr_tgt0))
+          (SIM: exists x, <<SIM: _simg r RR true f_tgt (ktr_src0 x) itr_tgt0>> /\ <<IH: P true f_tgt (ktr_src0 x) itr_tgt0>>),
+          P f_src f_tgt (trigger (Choose X) >>= ktr_src0) (itr_tgt0))
       (CHOOSER: forall
-          R0 R1 (RR: R0 -> R1 -> Prop) f_src f_tgt
+          f_src f_tgt
           X itr_src0 ktr_tgt0
           (CHOOSER: True)
-          (SIM: forall x, <<SIM: _simg r RR f_src true itr_src0 (ktr_tgt0 x)>> /\ <<IH: P _ _ RR f_src true itr_src0 (ktr_tgt0 x)>>),
-          P _ _ RR f_src f_tgt (itr_src0) (trigger (Choose X) >>= ktr_tgt0))
+          (SIM: forall x, <<SIM: _simg r RR f_src true itr_src0 (ktr_tgt0 x)>> /\ <<IH: P f_src true itr_src0 (ktr_tgt0 x)>>),
+          P f_src f_tgt (itr_src0) (trigger (Choose X) >>= ktr_tgt0))
       (TAKEL: forall
-          R0 R1 (RR: R0 -> R1 -> Prop) f_src f_tgt
+          f_src f_tgt
           X ktr_src0 itr_tgt0
           (TAKEL: True)
-          (SIM: forall x, <<SIM: _simg r RR true f_tgt (ktr_src0 x) itr_tgt0>> /\ <<IH: P _ _ RR true f_tgt (ktr_src0 x) itr_tgt0>>),
-          P _ _ RR f_src f_tgt (trigger (Take X) >>= ktr_src0) (itr_tgt0))
+          (SIM: forall x, <<SIM: _simg r RR true f_tgt (ktr_src0 x) itr_tgt0>> /\ <<IH: P true f_tgt (ktr_src0 x) itr_tgt0>>),
+          P f_src f_tgt (trigger (Take X) >>= ktr_src0) (itr_tgt0))
       (TAKER: forall
-          R0 R1 (RR: R0 -> R1 -> Prop) f_src f_tgt
+          f_src f_tgt
           X itr_src0 ktr_tgt0
           (TAKER: True)
-          (SIM: exists x, <<SIM: _simg r RR f_src true itr_src0 (ktr_tgt0 x)>> /\ <<IH: P _ _ RR f_src true itr_src0 (ktr_tgt0 x)>>),
-          P _ _ RR f_src f_tgt (itr_src0) (trigger (Take X) >>= ktr_tgt0))
+          (SIM: exists x, <<SIM: _simg r RR f_src true itr_src0 (ktr_tgt0 x)>> /\ <<IH: P f_src true itr_src0 (ktr_tgt0 x)>>),
+          P f_src f_tgt (itr_src0) (trigger (Take X) >>= ktr_tgt0))
       (PROGRESS: forall
-          R0 R1 (RR: R0 -> R1 -> Prop) f_src f_tgt
+          f_src f_tgt
           itr_src itr_tgt
           (SIM: r _ _ RR false false itr_src itr_tgt)
           (SRC: f_src = true)
           (TGT: f_tgt = true),
-          P _ _ RR f_src f_tgt itr_src itr_tgt)
+          P f_src f_tgt itr_src itr_tgt)
   :
-    forall R0 R1 (RR: R0 -> R1 -> Prop) f_src f_tgt itr_src itr_tgt
+    forall f_src f_tgt itr_src itr_tgt
            (SIM: _simg r RR f_src f_tgt itr_src itr_tgt),
-      P _ _ RR f_src f_tgt itr_src itr_tgt.
+      P f_src f_tgt itr_src itr_tgt.
 Proof.
-  fix IH 8. i. inv SIM.
+  fix IH 5. i. inv SIM.
   { eapply RET; eauto. }
   { eapply SYSCALL; eauto. }
   { eapply TAUL; eauto. }
@@ -270,66 +272,67 @@ Proof.
   { econs 9; eauto. eapply rclo7_base; eauto. }
 Qed.
 
-Lemma simg_ind (P: forall R0 R1 (RR: R0 -> R1 -> Prop), bool -> bool -> (itree eventE R0) -> (itree eventE R1) -> Prop)
+Lemma simg_ind R0 R1 (RR: R0 -> R1 -> Prop)
+      (P: bool -> bool -> (itree eventE R0) -> (itree eventE R1) -> Prop)
       (RET: forall
-          R0 R1 (RR: R0 -> R1 -> Prop) f_src f_tgt
+          f_src f_tgt
           r_src r_tgt
           (SIM: RR r_src r_tgt),
-          P _ _ RR f_src f_tgt (Ret r_src) (Ret r_tgt))
+          P f_src f_tgt (Ret r_src) (Ret r_tgt))
       (SYSCALL: forall
-          R0 R1 (RR: R0 -> R1 -> Prop) f_src f_tgt
+          f_src f_tgt
           ktr_src0 ktr_tgt0 fn varg rvs
           (SIM: forall x_src x_tgt (EQ: x_src = x_tgt), simg RR true true (ktr_src0 x_src) (ktr_tgt0 x_tgt)),
-          P _ _ RR f_src f_tgt (trigger (Syscall fn varg rvs) >>= ktr_src0) (trigger (Syscall fn varg rvs) >>= ktr_tgt0))
+          P f_src f_tgt (trigger (Syscall fn varg rvs) >>= ktr_src0) (trigger (Syscall fn varg rvs) >>= ktr_tgt0))
       (TAUL: forall
-          R0 R1 (RR: R0 -> R1 -> Prop) f_src f_tgt
+          f_src f_tgt
           itr_src0 itr_tgt0
           (TAUL: True)
           (SIM: simg RR true f_tgt itr_src0 itr_tgt0)
-          (IH: P _ _ RR true f_tgt itr_src0 itr_tgt0),
-          P _ _ RR f_src f_tgt (tau;; itr_src0) (itr_tgt0))
+          (IH: P true f_tgt itr_src0 itr_tgt0),
+          P f_src f_tgt (tau;; itr_src0) (itr_tgt0))
       (TAUR: forall
-          R0 R1 (RR: R0 -> R1 -> Prop) f_src f_tgt
+          f_src f_tgt
           itr_src0 itr_tgt0
           (TAUR: True)
           (SIM: simg RR f_src true itr_src0 itr_tgt0)
-          (IH: P _ _ RR f_src true itr_src0 itr_tgt0),
-          P _ _ RR f_src f_tgt (itr_src0) (tau;;itr_tgt0))
+          (IH: P f_src true itr_src0 itr_tgt0),
+          P f_src f_tgt (itr_src0) (tau;;itr_tgt0))
       (CHOOSEL: forall
-          R0 R1 (RR: R0 -> R1 -> Prop) f_src f_tgt
+          f_src f_tgt
           X ktr_src0 itr_tgt0
           (CHOOSEL: True)
-          (SIM: exists x, <<SIM: simg RR true f_tgt (ktr_src0 x) itr_tgt0>> /\ <<IH: P _ _ RR true f_tgt (ktr_src0 x) itr_tgt0>>),
-          P _ _ RR f_src f_tgt (trigger (Choose X) >>= ktr_src0) (itr_tgt0))
+          (SIM: exists x, <<SIM: simg RR true f_tgt (ktr_src0 x) itr_tgt0>> /\ <<IH: P true f_tgt (ktr_src0 x) itr_tgt0>>),
+          P f_src f_tgt (trigger (Choose X) >>= ktr_src0) (itr_tgt0))
       (CHOOSER: forall
-          R0 R1 (RR: R0 -> R1 -> Prop) f_src f_tgt
+          f_src f_tgt
           X itr_src0 ktr_tgt0
           (CHOOSER: True)
-          (SIM: forall x, <<SIM: simg RR f_src true itr_src0 (ktr_tgt0 x)>> /\ <<IH: P _ _ RR f_src true itr_src0 (ktr_tgt0 x)>>),
-          P _ _ RR f_src f_tgt (itr_src0) (trigger (Choose X) >>= ktr_tgt0))
+          (SIM: forall x, <<SIM: simg RR f_src true itr_src0 (ktr_tgt0 x)>> /\ <<IH: P f_src true itr_src0 (ktr_tgt0 x)>>),
+          P f_src f_tgt (itr_src0) (trigger (Choose X) >>= ktr_tgt0))
       (TAKEL: forall
-          R0 R1 (RR: R0 -> R1 -> Prop) f_src f_tgt
+          f_src f_tgt
           X ktr_src0 itr_tgt0
           (TAKEL: True)
-          (SIM: forall x, <<SIM: simg RR true f_tgt (ktr_src0 x) itr_tgt0>> /\ <<IH: P _ _ RR true f_tgt (ktr_src0 x) itr_tgt0>>),
-          P _ _ RR f_src f_tgt (trigger (Take X) >>= ktr_src0) (itr_tgt0))
+          (SIM: forall x, <<SIM: simg RR true f_tgt (ktr_src0 x) itr_tgt0>> /\ <<IH: P true f_tgt (ktr_src0 x) itr_tgt0>>),
+          P f_src f_tgt (trigger (Take X) >>= ktr_src0) (itr_tgt0))
       (TAKER: forall
-          R0 R1 (RR: R0 -> R1 -> Prop) f_src f_tgt
+          f_src f_tgt
           X itr_src0 ktr_tgt0
           (TAKER: True)
-          (SIM: exists x, <<SIM: simg RR f_src true itr_src0 (ktr_tgt0 x)>> /\ <<IH: P _ _ RR f_src true itr_src0 (ktr_tgt0 x)>>),
-          P _ _ RR f_src f_tgt (itr_src0) (trigger (Take X) >>= ktr_tgt0))
+          (SIM: exists x, <<SIM: simg RR f_src true itr_src0 (ktr_tgt0 x)>> /\ <<IH: P f_src true itr_src0 (ktr_tgt0 x)>>),
+          P f_src f_tgt (itr_src0) (trigger (Take X) >>= ktr_tgt0))
       (PROGRESS: forall
-          R0 R1 (RR: R0 -> R1 -> Prop) f_src f_tgt
+          f_src f_tgt
           itr_src itr_tgt
           (SIM: simg RR false false itr_src itr_tgt)
           (SRC: f_src = true)
           (TGT: f_tgt = true),
-          P _ _ RR f_src f_tgt itr_src itr_tgt)
+          P f_src f_tgt itr_src itr_tgt)
   :
-    forall R0 R1 (RR: R0 -> R1 -> Prop) f_src f_tgt itr_src itr_tgt
+    forall f_src f_tgt itr_src itr_tgt
            (SIM: simg RR f_src f_tgt itr_src itr_tgt),
-      P _ _ RR f_src f_tgt itr_src itr_tgt.
+      P f_src f_tgt itr_src itr_tgt.
 Proof.
   i. punfold SIM. induction SIM using _simg_ind2; i; clarify.
   { eapply RET; eauto. }
@@ -434,7 +437,7 @@ Lemma grespectful7'_grespectful7
 Proof.
 Abort.
 
-Lemma sim_progress R0 R1 RR r g itr_src itr_tgt
+Lemma simg_progress_flag R0 R1 RR r g itr_src itr_tgt
       (SIM: gpaco7 _simg (cpn7 _simg) g g R0 R1 RR false false itr_src itr_tgt)
   :
     gpaco7 _simg (cpn7 _simg) r g R0 R1 RR true true itr_src itr_tgt.
@@ -642,567 +645,41 @@ Proof.
   generalize itr_tgt at 1 as md_tgt.
   generalize itr_src at 1 as md_src. i. ginit.
   revert o_src0 o_tgt0 itr_src itr_tgt SIMG. gcofix CIH.
-  i. induction SIMG using simg_ind. punfold SIMG. inv SIMG; pfold.
-
-
-  unfold Beh.of_program. ss.
-  i. destruct SIM as [o_src0 [o_tgt0 SIMG]].
-  remember itr_tgt in PR.
-  revert Heqi o_src0 o_tgt0 SIMG. punfold PR. inv PR; ss.
-
-  inv PR.
-
-  induction PR.
-
-  revert x0.
-
-  Set Printing All.
-  remember (@ModSemL.compile_itree CONFT itr_tgt) in PR.
-
-
-  eapply adequacy_aux; et.
-  { eapply Ord.lt_well_founded. }
-  { eapply Ord.lt_well_founded. }
-  instantiate (1:=o_tgt0). instantiate (1:=o_src0). clear x0 PR.
-  generalize itr_tgt at 1 as md_tgt.
-  generalize itr_src at 1 as md_src. i.
-  revert o_src0 o_tgt0 itr_src itr_tgt SIMG. pcofix CIH.
-  i. punfold SIMG. inv SIMG; pfold.
-  { destruct (finalize r_tgt) eqn:T.
+  i. induction SIMG using simg_ind; i; clarify.
+  { gstep. destruct (finalize r_tgt) eqn:T.
     { eapply sim_fin; ss; cbn; des_ifs; rewrite FINSAME in *; clarify. }
     { eapply sim_angelic_src.
       { cbn. des_ifs; rewrite FINSAME in *; clarify. }
       i. exfalso. inv STEP.
     }
   }
-  { eapply sim_vis; ss. i.
+  { gstep. eapply sim_vis; ss. i.
     eapply step_trigger_syscall_iff in STEP. des. clarify.
     esplits.
     { eapply step_trigger_syscall; et. }
-    { right. eapply CIH.
-      hexploit SIM; et. i. pclearbot. eapply H. }
+    { gbase. eapply CIH. hexploit SIM; et. }
   }
-  { eapply sim_demonic_src; ss.
-    esplits.
-    { eapply step_tau; et. }
-    { et. }
-    { right. eapply CIH. destruct SIM; ss. et. }
+  { guclo sim_indC_spec. eapply sim_indC_demonic_src; ss.
+    esplits; eauto. eapply step_tau; et.
   }
-  { eapply sim_demonic_tgt; ss. i.
+  { guclo sim_indC_spec. eapply sim_indC_demonic_tgt; ss. i.
     eapply step_tau_iff in STEP. des. clarify.
-    esplits.
-    { et. }
-    { right. eapply CIH. destruct SIM; ss. et. }
   }
-  { eapply sim_demonic_src; ss. destruct SIM.
-    esplits.
-    { eapply step_trigger_choose; et. }
-    { et. }
-    { right. eapply CIH. destruct H; ss. apply p. }
+  { des. guclo sim_indC_spec. eapply sim_indC_demonic_src; ss.
+    esplits; eauto. eapply step_trigger_choose; et.
   }
-  { eapply sim_demonic_tgt; ss. i.
-    eapply step_trigger_choose_iff in STEP. des. clarify.
-    hexploit (SIM x); et. i. des.
-    esplits.
-    { et. }
-    { right. eapply CIH. destruct H; ss. et. }
+  { guclo sim_indC_spec. eapply sim_indC_demonic_tgt; ss.
+    i.  eapply step_trigger_choose_iff in STEP. des. clarify.
+    hexploit (SIM x); et. i. des. esplits; eauto.
   }
-  { eapply sim_angelic_src; ss. i.
+  { guclo sim_indC_spec. eapply sim_indC_angelic_src; ss. i.
     eapply step_trigger_take_iff in STEP. des. clarify.
-    hexploit (SIM x); et. i. des.
-    esplits.
-    { et. }
-    { right. eapply CIH. destruct H; ss. et. }
+    hexploit (SIM x); et. i. des. esplits; et.
   }
-  { eapply sim_angelic_tgt; ss. destruct SIM.
-    esplits.
-    { eapply step_trigger_take; et. }
-    { et. }
-    { right. eapply CIH. destruct H; ss. apply p. }
+  { des. guclo sim_indC_spec. eapply sim_indC_angelic_tgt; ss.
+    esplits; eauto. eapply step_trigger_take; et.
   }
-Qed.
-
-
-Variable md_src md_tgt: ModL.t.
-Let ms_src: ModSemL.t := md_src.(ModL.enclose).
-Let ms_tgt: ModSemL.t := md_tgt.(ModL.enclose).
-
-Section ADEQUACY.
-Hypothesis (SIM: exists o_src0 o_tgt0, simg eq o_src0 o_tgt0 (@ModSemL.initial_itr ms_src CONFS (Some (ModL.wf md_src))) (@ModSemL.initial_itr ms_tgt CONFT (Some (ModL.wf md_tgt)))).
-
-
-Theorem adequacy_global: Beh.of_program (@ModL.compile _ CONFT md_tgt) <1= Beh.of_program (@ModL.compile _ CONFS md_src).
-Proof.
-  eapply adequacy_global_itree. eapply SIM.
-Qed.
-End ADEQUACY.
-End SIM.
-
-
-
-Theorem simg_bind
-        R0 R1 S0 S1
-        RR SS
-        o_src0 o_tgt0 (itr_src: itree eventE R0) (itr_tgt: itree eventE R1)
-        (SIM: simg RR o_src0 o_tgt0 itr_src itr_tgt)
-        o_src1 o_tgt1 (ktr_src: ktree eventE R0 S0) (ktr_tgt: ktree eventE R1 S1)
-        (SIMK: forall vret_src vret_tgt (SIM: RR vret_src vret_tgt), simg SS o_src1 o_tgt1 (ktr_src vret_src) (ktr_tgt vret_tgt))
-  :
-    simg SS (OrdArith.add o_src1 o_src0) (OrdArith.add o_tgt1 o_tgt0)
-         (itr_src >>= ktr_src) (itr_tgt >>= ktr_tgt)
-.
-Proof.
-  ginit.
-  { eapply cpn7_wcompat; eauto with paco. }
-  guclo bindC_spec. econs.
-  - eauto with paco.
-  - ii. exploit SIMK; eauto with paco.
-Qed.
-
-
-
-
-
-
-
-
-
-
-
-
-
-
-
-Variant ordC (r: forall S0 S1 (SS: S0 -> S1 -> Prop), Ord.t -> Ord.t -> (itree eventE S0) -> (itree eventE S1) -> Prop):
-  forall S0 S1 (SS: S0 -> S1 -> Prop), Ord.t -> Ord.t -> (itree eventE S0) -> (itree eventE S1) -> Prop :=
-| ordC_intro
-    o_src0 o_src1 o_tgt0 o_tgt1 R0 R1 (RR: R0 -> R1 -> Prop) itr_src itr_tgt
-    (ORDSRC: Ord.le o_src0 o_src1)
-    (ORDTGT: Ord.le o_tgt0 o_tgt1)
-    (SIM: r _ _ RR o_src0 o_tgt0 itr_src itr_tgt)
-  :
-    ordC r RR o_src1 o_tgt1 itr_src itr_tgt
-.
-Hint Constructors ordC: core.
-
-Lemma ordC_mon
-      r1 r2
-      (LE: r1 <7= r2)
-  :
-    ordC r1 <7= ordC r2
-.
-Proof. ii. destruct PR; econs; et. Qed.
-Hint Resolve ordC_mon: paco.
-
-Lemma ordC_prespectful: prespectful7 (_simg) ordC.
-Proof.
-  econs; eauto with paco.
-  ii. inv PR. csc.
-  rename x2 into o1. apply GF in SIM. pfold. inv SIM.
-  - econs; eauto.
-  - econs; eauto.
-  - econs; eauto. { eapply Ord.lt_le_lt; et. }
-  - econs; eauto. { eapply Ord.lt_le_lt; et. }
-  - econs; eauto. { eapply Ord.lt_le_lt; et. } des. esplits; et.
-  - econs; eauto. { eapply Ord.lt_le_lt; et. }
-  - econs; eauto. { eapply Ord.lt_le_lt; et. }
-  - econs; eauto. { eapply Ord.lt_le_lt; et. } des. esplits; et.
-Qed.
-
-Lemma ordC_spec: ordC <8= gupaco7 (_simg) (cpn7 _simg).
-Proof. intros. eapply prespect7_uclo; eauto with paco. eapply ordC_prespectful. Qed.
-
-Global Program Instance simg_paco_refl r R RR `{Reflexive _ RR}
-  : Reflexive (paco7 _simg r R R RR o_src0 o_tgt0).
-Next Obligation.
-  revert_until r. pcofix CIH. i. pfold. ides x.
-  - econs; et.
-  - econs 3; et. left. pfold. econs 4; auto.
-    { eapply Ord.S_lt. }
-    right. et.
-  - rewrite <- ! bind_trigger. destruct e.
-    + econs 6; et. i. left. pfold. econs 5; auto.
-      { eapply Ord.S_lt. }
-      esplits. right. et.
-    + econs 7; et. i. left. pfold. econs 8; auto.
-      { eapply Ord.S_lt. }
-      esplits. right. et.
-    + econs; et. i. subst. right. et.
-Qed.
-
-Global Program Instance simg_gpaco_refl r R RR `{Reflexive _ RR} rg o_src0 o_tgt0
-       (LT: Ord.lt Ord.O o_src0 /\ Ord.lt Ord.O o_tgt0)
-  : Reflexive (gpaco7 _simg (cpn7 _simg) r rg R R RR o_src0 o_tgt0).
-Next Obligation.
-  gfinal. right. eapply simg_paco_refl; et.
-Qed.
-
-Global Program Instance simg_refl R RR `{Reflexive _ RR} o_src0 o_tgt0
-       (LT: Ord.lt Ord.O o_src0 /\ Ord.lt Ord.O o_tgt0)
-  : Reflexive (@simg R R RR o_src0 o_tgt0).
-Next Obligation.
-  eapply simg_paco_refl; ss.
-Qed.
-
-
-
-
-
-
-
-
-
-
-
-
-
-
-
-
-
-
-
-
-
-
-Variant ordC (r: forall S0 S1 (SS: S0 -> S1 -> Prop), Ord.t -> Ord.t -> (itree eventE S0) -> (itree eventE S1) -> Prop):
-  forall S0 S1 (SS: S0 -> S1 -> Prop), Ord.t -> Ord.t -> (itree eventE S0) -> (itree eventE S1) -> Prop :=
-| ordC_intro
-    o_src0 o_src1 o_tgt0 o_tgt1 R0 R1 (RR: R0 -> R1 -> Prop) itr_src itr_tgt
-    (ORDSRC: Ord.le o_src0 o_src1)
-    (ORDTGT: Ord.le o_tgt0 o_tgt1)
-    (SIM: r _ _ RR o_src0 o_tgt0 itr_src itr_tgt)
-  :
-    ordC r RR o_src1 o_tgt1 itr_src itr_tgt
-.
-Hint Constructors ordC: core.
-
-Lemma ordC_mon
-      r1 r2
-      (LE: r1 <7= r2)
-  :
-    ordC r1 <7= ordC r2
-.
-Proof. ii. destruct PR; econs; et. Qed.
-Hint Resolve ordC_mon: paco.
-
-Lemma ordC_prespectful: prespectful7 (_simg) ordC.
-Proof.
-  econs; eauto with paco.
-  ii. inv PR. csc.
-  rename x2 into o1. apply GF in SIM. pfold. inv SIM.
-  - econs; eauto.
-  - econs; eauto.
-  - econs; eauto. { eapply Ord.lt_le_lt; et. }
-  - econs; eauto. { eapply Ord.lt_le_lt; et. }
-  - econs; eauto. { eapply Ord.lt_le_lt; et. } des. esplits; et.
-  - econs; eauto. { eapply Ord.lt_le_lt; et. }
-  - econs; eauto. { eapply Ord.lt_le_lt; et. }
-  - econs; eauto. { eapply Ord.lt_le_lt; et. } des. esplits; et.
-Qed.
-
-Lemma ordC_spec: ordC <8= gupaco7 (_simg) (cpn7 _simg).
-Proof. intros. eapply prespect7_uclo; eauto with paco. eapply ordC_prespectful. Qed.
-
-
-
-
-
-
-
-
-
-
-
-Variant bindR (r s: forall S0 S1 (SS: S0 -> S1 -> Prop), Ord.t -> Ord.t -> (itree eventE S0) -> (itree eventE S1) -> Prop):
-  forall S0 S1 (SS: S0 -> S1 -> Prop), Ord.t -> Ord.t -> (itree eventE S0) -> (itree eventE S1) -> Prop :=
-| bindR_intro
-    o_src0 o_src1 o_tgt0 o_tgt1
-
-    R0 R1 RR
-    (i_src: itree eventE R0) (i_tgt: itree eventE R1)
-    (SIM: r _ _ RR o_src0 o_tgt0 i_src i_tgt)
-
-    S0 S1 SS
-    (k_src: ktree eventE R0 S0) (k_tgt: ktree eventE R1 S1)
-    (SIMK: forall vret_src vret_tgt (SIM: RR vret_src vret_tgt), s _ _ SS o_src1 o_tgt1 (k_src vret_src) (k_tgt vret_tgt))
-  :
-    (* bindR r s (Ordinal.add o0 o1) (ITree.bind i_src k_src) (ITree.bind i_tgt k_tgt) *)
-    bindR r s SS (OrdArith.add o_src1 o_src0) (OrdArith.add o_tgt1 o_tgt0) (ITree.bind i_src k_src) (ITree.bind i_tgt k_tgt)
-.
-
-Hint Constructors bindR: core.
-
-Lemma bindR_mon
-      r1 r2 s1 s2
-      (LEr: r1 <7= r2) (LEs: s1 <7= s2)
-  :
-    bindR r1 s1 <7= bindR r2 s2
-.
-Proof. ii. destruct PR; econs; et. Qed.
-
-Definition bindC r := bindR r r.
-Hint Unfold bindC: core.
-
-Lemma bindC_wrespectful: wrespectful7 (_simg) bindC.
-Proof.
-  econstructor; repeat intro.
-  { eapply bindR_mon; eauto. }
-  rename l into llll.
-  eapply bindR_mon in PR; cycle 1.
-  { eapply GF. }
-  { i. eapply PR0. }
-  inv PR. csc. inv SIM.
-  + irw.
-    exploit SIMK; eauto. i.
-    eapply simg_mon_ord.
-    { eapply OrdArith.add_base_l. }
-    { eapply OrdArith.add_base_l. }
-    eapply simg_mon; eauto with paco.
-  + rewrite ! bind_bind. econs; eauto. ii.
-    { econs 2; eauto with paco. econs; eauto with paco. }
-
-  + rewrite ! bind_tau. econs; eauto.
-    { eapply OrdArith.lt_add_r; et. }
-    econs 2; eauto with paco. econs; eauto with paco.
-  + irw. econs; eauto.
-    { eapply OrdArith.lt_add_r; et. }
-    econs 2; eauto with paco. econs; eauto with paco.
-
-  + rewrite ! bind_bind. econs; eauto.
-    { eapply OrdArith.lt_add_r; et. }
-    des. esplits; et. econs 2; eauto with paco. econs; eauto with paco.
-  + rewrite ! bind_bind. econs; eauto.
-    { eapply OrdArith.lt_add_r; et. }
-    des. esplits; et. econs 2; eauto with paco. econs; eauto with paco.
-
-  + rewrite ! bind_bind. econs; eauto.
-    { eapply OrdArith.lt_add_r; et. }
-    des. esplits; et. econs 2; eauto with paco. econs; eauto with paco.
-  + rewrite ! bind_bind. econs; eauto.
-    { eapply OrdArith.lt_add_r; et. }
-    des. esplits; et. econs 2; eauto with paco. econs; eauto with paco.
-Qed.
-
-Lemma bindC_spec: bindC <8= gupaco7 (_simg) (cpn7 (_simg)).
-Proof.
-  intros. eapply wrespect7_uclo; eauto with paco. eapply bindC_wrespectful.
-Qed.
-
-Theorem simg_bind
-        R0 R1 S0 S1
-        RR SS
-        o_src0 o_tgt0 (itr_src: itree eventE R0) (itr_tgt: itree eventE R1)
-        (SIM: simg RR o_src0 o_tgt0 itr_src itr_tgt)
-        o_src1 o_tgt1 (ktr_src: ktree eventE R0 S0) (ktr_tgt: ktree eventE R1 S1)
-        (SIMK: forall vret_src vret_tgt (SIM: RR vret_src vret_tgt), simg SS o_src1 o_tgt1 (ktr_src vret_src) (ktr_tgt vret_tgt))
-  :
-    simg SS (OrdArith.add o_src1 o_src0) (OrdArith.add o_tgt1 o_tgt0)
-         (itr_src >>= ktr_src) (itr_tgt >>= ktr_tgt)
-.
-Proof.
-  ginit.
-  { eapply cpn7_wcompat; eauto with paco. }
-  guclo bindC_spec. econs.
-  - eauto with paco.
-  - ii. exploit SIMK; eauto with paco.
-Qed.
-
-
-
-Lemma step_trigger_choose_iff X k itr e
-      (STEP: ModSemL.step (trigger (Choose X) >>= k) e itr)
-  :
-    exists x,
-      e = None /\ itr = k x.
-Proof.
-  inv STEP.
-  { eapply f_equal with (f:=observe) in H0. ss. }
-  { eapply f_equal with (f:=observe) in H0. ss.
-    unfold trigger in H0. ss. cbn in H0.
-    dependent destruction H0. ired. et.  }
-  { eapply f_equal with (f:=observe) in H0. ss. }
-  { eapply f_equal with (f:=observe) in H0. ss. }
-Qed.
-
-Lemma step_trigger_take_iff X k itr e
-      (STEP: ModSemL.step (trigger (Take X) >>= k) e itr)
-  :
-    exists x,
-      e = None /\ itr = k x.
-Proof.
-  inv STEP.
-  { eapply f_equal with (f:=observe) in H0. ss. }
-  { eapply f_equal with (f:=observe) in H0. ss. }
-  { eapply f_equal with (f:=observe) in H0. ss.
-    unfold trigger in H0. ss. cbn in H0.
-    dependent destruction H0. ired. et.  }
-  { eapply f_equal with (f:=observe) in H0. ss. }
-Qed.
-
-Lemma step_tau_iff itr0 itr1 e
-      (STEP: ModSemL.step (Tau itr0) e itr1)
-  :
-    e = None /\ itr0 = itr1.
-Proof.
-  inv STEP. et.
-Qed.
-
-Lemma step_ret_iff rv itr e
-      (STEP: ModSemL.step (Ret rv) e itr)
-  :
-    False.
-Proof.
-  inv STEP.
-Qed.
-
-Lemma step_trigger_syscall_iff fn args rvs k e itr
-      (STEP: ModSemL.step (trigger (Syscall fn args rvs) >>= k) e itr)
-  :
-    exists rv, itr = k rv /\ e = Some (event_sys fn args rv)
-               /\ <<RV: rvs rv>> /\ <<SYS: syscall_sem (event_sys fn args rv)>>.
-Proof.
-  inv STEP.
-  { eapply f_equal with (f:=observe) in H0. ss. }
-  { eapply f_equal with (f:=observe) in H0. ss. }
-  { eapply f_equal with (f:=observe) in H0. ss. }
-  { eapply f_equal with (f:=observe) in H0. ss.
-    unfold trigger in H0. ss. cbn in H0.
-    dependent destruction H0. ired. et. }
-Qed.
-
-
-Lemma itree_eta_eq E R (itr0 itr1: itree E R)
-    (OBSERVE: observe itr0 = observe itr1)
-  :
-    itr0 = itr1.
-Proof.
-  rewrite (itree_eta_ itr0).
-  rewrite (itree_eta_ itr1).
-  rewrite OBSERVE. auto.
-Qed.
-
-Lemma step_trigger_choose X k x
-  :
-    ModSemL.step (trigger (Choose X) >>= k) None (k x).
-Proof.
-  unfold trigger. ss.
-  match goal with
-  | [ |- ModSemL.step ?itr _ _] =>
-    replace itr with (Subevent.vis (Choose X) k)
-  end; ss.
-  { econs. }
-  { eapply itree_eta_eq. ss. cbv. f_equal.
-    extensionality x0. eapply itree_eta_eq. ss. }
-Qed.
-
-Lemma step_trigger_take X k x
-  :
-    ModSemL.step (trigger (Take X) >>= k) None (k x).
-Proof.
-  unfold trigger. ss.
-  match goal with
-  | [ |- ModSemL.step ?itr _ _] =>
-    replace itr with (Subevent.vis (Take X) k)
-  end; ss.
-  { econs. }
-  { eapply itree_eta_eq. ss. cbv. f_equal.
-    extensionality x0. eapply itree_eta_eq. ss. }
-Qed.
-
-Lemma step_trigger_syscall fn args (rvs: Any.t -> Prop) k rv
-      (RV: rvs rv) (SYS: syscall_sem (event_sys fn args rv))
-  :
-    ModSemL.step (trigger (Syscall fn args rvs) >>= k) (Some (event_sys fn args rv)) (k rv).
-Proof.
-  unfold trigger. ss.
-  match goal with
-  | [ |- ModSemL.step ?itr _ _] =>
-    replace itr with (Subevent.vis (Syscall fn args rvs) k)
-  end; ss.
-  { econs; et. }
-  { eapply itree_eta_eq. ss. cbv. f_equal.
-    extensionality x0. eapply itree_eta_eq. ss. }
-Qed.
-
-Lemma step_tau itr
-  :
-    ModSemL.step (Tau itr) None itr.
-Proof.
-  econs.
-Qed.
-
-Context {CONFS CONFT: EMSConfig}.
-Hypothesis (FINSAME: (@finalize CONFS) = (@finalize CONFT)).
-
-Theorem adequacy_global_itree itr_src itr_tgt
-        (SIM: exists o_src0 o_tgt0, simg eq o_src0 o_tgt0 itr_src itr_tgt)
-  :
-    Beh.of_program (@ModSemL.compile_itree CONFT itr_tgt)
-    <1=
-    Beh.of_program (@ModSemL.compile_itree CONFS itr_src).
-Proof.
-  unfold Beh.of_program. ss.
-  i. destruct SIM as [o_src0 [o_tgt0 SIMG]]. eapply adequacy_aux; et.
-  { eapply Ord.lt_well_founded. }
-  { eapply Ord.lt_well_founded. }
-  instantiate (1:=o_tgt0). instantiate (1:=o_src0). clear x0 PR.
-  generalize itr_tgt at 1 as md_tgt.
-  generalize itr_src at 1 as md_src. i.
-  revert o_src0 o_tgt0 itr_src itr_tgt SIMG. pcofix CIH.
-  i. punfold SIMG. inv SIMG; pfold.
-  { destruct (finalize r_tgt) eqn:T.
-    { eapply sim_fin; ss; cbn; des_ifs; rewrite FINSAME in *; clarify. }
-    { eapply sim_angelic_src.
-      { cbn. des_ifs; rewrite FINSAME in *; clarify. }
-      i. exfalso. inv STEP.
-    }
-  }
-  { eapply sim_vis; ss. i.
-    eapply step_trigger_syscall_iff in STEP. des. clarify.
-    esplits.
-    { eapply step_trigger_syscall; et. }
-    { right. eapply CIH.
-      hexploit SIM; et. i. pclearbot. eapply H. }
-  }
-  { eapply sim_demonic_src; ss.
-    esplits.
-    { eapply step_tau; et. }
-    { et. }
-    { right. eapply CIH. destruct SIM; ss. et. }
-  }
-  { eapply sim_demonic_tgt; ss. i.
-    eapply step_tau_iff in STEP. des. clarify.
-    esplits.
-    { et. }
-    { right. eapply CIH. destruct SIM; ss. et. }
-  }
-  { eapply sim_demonic_src; ss. destruct SIM.
-    esplits.
-    { eapply step_trigger_choose; et. }
-    { et. }
-    { right. eapply CIH. destruct H; ss. apply p. }
-  }
-  { eapply sim_demonic_tgt; ss. i.
-    eapply step_trigger_choose_iff in STEP. des. clarify.
-    hexploit (SIM x); et. i. des.
-    esplits.
-    { et. }
-    { right. eapply CIH. destruct H; ss. et. }
-  }
-  { eapply sim_angelic_src; ss. i.
-    eapply step_trigger_take_iff in STEP. des. clarify.
-    hexploit (SIM x); et. i. des.
-    esplits.
-    { et. }
-    { right. eapply CIH. destruct H; ss. et. }
-  }
-  { eapply sim_angelic_tgt; ss. destruct SIM.
-    esplits.
-    { eapply step_trigger_take; et. }
-    { et. }
-    { right. eapply CIH. destruct H; ss. apply p. }
-  }
+  { gstep. eapply sim_progress; eauto. gbase. auto. }
 Qed.
 
 
@@ -1224,662 +701,64 @@ End SIM.
 Hint Constructors _simg.
 Hint Unfold simg.
 Hint Resolve simg_mon: paco.
-Hint Constructors ordC: core.
-Hint Resolve ordC_mon: paco.
+Hint Constructors flagC: core.
+Hint Resolve flagC_mon: paco.
 Hint Constructors bindR: core.
 Hint Unfold bindC: core.
+Hint Constructors simg_indC: core.
+Hint Resolve sim_indC_mon: paco.
 
 
-Inductive _simg_safe (simg: forall R0 R1 (RR: R0 -> R1 -> Prop), Ord.t -> Ord.t -> (itree eventE R0) -> (itree eventE R1) -> Prop)
-          {R0 R1} (RR: R0 -> R1 -> Prop) (i_src0 i_tgt0: Ord.t): (itree eventE R0) -> (itree eventE R1) -> Prop :=
+Variant _simg_safe
+          (simg: forall R0 R1 (RR: R0 -> R1 -> Prop), bool -> bool -> (itree eventE R0) -> (itree eventE R1) -> Prop)
+          {R0 R1} (RR: R0 -> R1 -> Prop) (f_src f_tgt: bool): (itree eventE R0) -> (itree eventE R1) -> Prop :=
 | simg_safe_ret
     r_src r_tgt
     (SIM: RR r_src r_tgt)
   :
-    _simg_safe simg RR i_src0 i_tgt0 (Ret r_src) (Ret r_tgt)
+    _simg_safe simg RR f_src f_tgt (Ret r_src) (Ret r_tgt)
 | simg_safe_syscall
-    i_src1 i_tgt1 ktr_src0 ktr_tgt0 fn varg rvs
-    (SIM: forall x_src x_tgt (EQ: x_src = x_tgt), simg _ _ RR i_src1 i_tgt1 (ktr_src0 x_src) (ktr_tgt0 x_tgt))
+    ktr_src0 ktr_tgt0 fn varg rvs
+    (SIM: forall x_src x_tgt (EQ: x_src = x_tgt), simg _ _ RR true true (ktr_src0 x_src) (ktr_tgt0 x_tgt))
   :
-    _simg_safe simg RR i_src0 i_tgt0 (trigger (Syscall fn varg rvs) >>= ktr_src0) (trigger (Syscall fn varg rvs) >>= ktr_tgt0)
-
+    _simg_safe simg RR f_src f_tgt (trigger (Syscall fn varg rvs) >>= ktr_src0) (trigger (Syscall fn varg rvs) >>= ktr_tgt0)
 
 | simg_safe_tauL
-    i_src1 i_tgt1 itr_src0 itr_tgt0
+    itr_src0 itr_tgt0
     (TAUL: True)
-    (ORD: Ord.lt i_tgt1 i_tgt0)
-    (SIM: simg _ _ RR i_src1 i_tgt1 itr_src0 itr_tgt0)
+    (SIM: simg _ _ RR true f_tgt itr_src0 itr_tgt0)
   :
-    _simg_safe simg RR i_src0 i_tgt0 (tau;; itr_src0) (itr_tgt0)
+    _simg_safe simg RR f_src f_tgt (tau;; itr_src0) (itr_tgt0)
 | simg_safe_tauR
-    i_src1 i_tgt1 itr_src0 itr_tgt0
+    itr_src0 itr_tgt0
     (TAUR: True)
-    (ORD: Ord.lt i_src1 i_src0)
-    (SIM: simg _ _ RR i_src1 i_tgt1 itr_src0 itr_tgt0)
+    (SIM: simg _ _ RR f_src true itr_src0 itr_tgt0)
   :
-    _simg_safe simg RR i_src0 i_tgt0 (itr_src0) (tau;; itr_tgt0)
-
+    _simg_safe simg RR f_src f_tgt (itr_src0) (tau;; itr_tgt0)
 
 | simg_safe_chooseR
-    i_src1 i_tgt1 X itr_src0 ktr_tgt0
+    X itr_src0 ktr_tgt0
     (CHOOSER: True)
-    (ORD: Ord.lt i_src1 i_src0)
-    (SIM: forall x, simg _ _ RR i_src1 i_tgt1 itr_src0 (ktr_tgt0 x))
+    (SIM: forall x, simg _ _ RR f_src true itr_src0 (ktr_tgt0 x))
   :
-    _simg_safe simg RR i_src0 i_tgt0 (itr_src0) (trigger (Choose X) >>= ktr_tgt0)
-
+    _simg_safe simg RR f_src f_tgt (itr_src0) (trigger (Choose X) >>= ktr_tgt0)
 
 | simg_safe_takeL
-    i_src1 i_tgt1 X ktr_src0 itr_tgt0
+    X ktr_src0 itr_tgt0
     (TAKEL: True)
-    (ORD: Ord.lt i_tgt1 i_tgt0)
-    (SIM: forall x, simg _ _ RR i_src1 i_tgt1 (ktr_src0 x) itr_tgt0)
+    (SIM: forall x, simg _ _ RR true f_tgt (ktr_src0 x) itr_tgt0)
   :
-    _simg_safe simg RR i_src0 i_tgt0 (trigger (Take X) >>= ktr_src0) (itr_tgt0)
+    _simg_safe simg RR f_src f_tgt (trigger (Take X) >>= ktr_src0) (itr_tgt0)
 .
 
 Lemma simg_safe_spec:
-  _simg_safe <8= _simg.
-Proof. i. inv PR; try by (econs; eauto). Qed.
-
-Section TY.
-(* Context `{R: Type}. *)
-Inductive _simg (simg: forall R0 R1 (RR: R0 -> R1 -> Prop), bool -> bool -> (itree eventE R0) -> (itree eventE R1) -> Prop)
-          {R0 R1} (RR: R0 -> R1 -> Prop) (i_src0 i_tgt0: bool): (itree eventE R0) -> (itree eventE R1) -> Prop :=
-| simg_ret
-    r_src r_tgt
-    (SIM: RR r_src r_tgt)
-  :
-    _simg simg RR i_src0 i_tgt0 (Ret r_src) (Ret r_tgt)
-| simg_syscall
-    i_src1 i_tgt1 ktr_src0 ktr_tgt0 fn varg rvs
-    (SIM: forall x_src x_tgt (EQ: x_src = x_tgt), simg _ _ RR i_src1 i_tgt1 (ktr_src0 x_src) (ktr_tgt0 x_tgt))
-  :
-    _simg simg RR i_src0 i_tgt0 (trigger (Syscall fn varg rvs) >>= ktr_src0) (trigger (Syscall fn varg rvs) >>= ktr_tgt0)
-
-
-| simg_tauL
-    i_tgt1 itr_src0 itr_tgt0
-    (TAUL: True)
-    (SIM: @_simg simg _ _ RR i_src0 i_tgt1 itr_src0 itr_tgt0)
-  :
-    _simg simg RR i_src0 i_tgt0 (tau;; itr_src0) (itr_tgt0)
-| simg_tauR
-    i_src1 itr_src0 itr_tgt0
-    (TAUR: True)
-    (SIM: @_simg simg _ _ RR i_src1 i_tgt0 itr_src0 itr_tgt0)
-  :
-    _simg simg RR i_src0 i_tgt0 (itr_src0) (tau;; itr_tgt0)
-
-
-| simg_chooseL
-    i_tgt1 X ktr_src0 itr_tgt0
-    (CHOOSEL: True)
-    (SIM: exists x, @_simg simg _ _ RR i_src0 i_tgt1 (ktr_src0 x) itr_tgt0)
-  :
-    _simg simg RR i_src0 i_tgt0 (trigger (Choose X) >>= ktr_src0) (itr_tgt0)
-| simg_chooseR
-    i_src1 X itr_src0 ktr_tgt0
-    (CHOOSER: True)
-    (SIM: forall x, @_simg simg _ _ RR i_src1 i_tgt0 itr_src0 (ktr_tgt0 x))
-  :
-    _simg simg RR i_src0 i_tgt0 (itr_src0) (trigger (Choose X) >>= ktr_tgt0)
-
-
-| simg_takeL
-    i_tgt1 X ktr_src0 itr_tgt0
-    (TAKEL: True)
-    (SIM: forall x, @_simg simg _ _ RR i_src0 i_tgt1 (ktr_src0 x) itr_tgt0)
-  :
-    _simg simg RR i_src0 i_tgt0 (trigger (Take X) >>= ktr_src0) (itr_tgt0)
-| simg_takeR
-    i_src1 X itr_src0 ktr_tgt0
-    (TAKER: True)
-    (SIM: exists x, @_simg simg _ _ RR i_src1 i_tgt0 itr_src0 (ktr_tgt0 x))
-  :
-    _simg simg RR i_src0 i_tgt0 (itr_src0) (trigger (Take X) >>= ktr_tgt0)
-
-
-| simg_progress
-    itr_src itr_tgt
-    (SIM: simg _ _ RR false false itr_src itr_tgt)
-    (SRC: i_src0 = true)
-    (TGT: i_tgt0 = true)
-  :
-    _simg simg RR i_src0 i_tgt0 itr_src itr_tgt
-.
-
-Definition simg: forall R0 R1 (RR: R0 -> R1 -> Prop), bool -> bool -> (itree eventE R0) -> (itree eventE R1) -> Prop := paco7 _simg bot7.
-
-Lemma simg_mon: monotone7 _simg.
+  _simg_safe <8= gupaco7 _simg (cpn7 _simg).
 Proof.
-  ii. induction IN.
-  { econs 1; eauto. }
-  { econs 2; eauto. }
-  { econs 3; eauto. }
-  { econs 4; eauto. }
-Admitted.
-  { des. econs 5; eauto. esplits; et. }
-  { econs 3; eauto. }
-  { econs 3; eauto. }
-  { econs 3; eauto. }
-  { econs 1; eauto. }
-  { econs 1; eauto. }
-  { econs 1; eauto. }
-  { econs 1; eauto. }
-  { econs 1; eauto. }
-
- inv IN; try (by econs; et).
-  - econs; et. ii. hexploit SIM; et. i; des. esplits; et.
-  - des. econs; et.
+  i. eapply simg_indC_spec. inv PR.
+  { econs; eauto. }
+  { econs; eauto. }
+  { econs; eauto. }
+  { econs; eauto. }
+  { econs; eauto. }
+  { econs; eauto. }
 Qed.
-
-Lemma simg_mon_ord r S0 S1 SS i_src0 i_src1 i_tgt0 i_tgt1
-      (ORDSRC: Ord.le i_src0 i_src1) (ORDTGT: Ord.le i_tgt0 i_tgt1):
-  @_simg r S0 S1 SS i_src0 i_tgt0 <2= @_simg r S0 S1 SS i_src1 i_tgt1.
-Proof.
-  ii. inv PR; try (by econs; et).
-  (* - econs; try apply SIM; et. etrans; et. *)
-  - econs; try apply SIM; et. eapply Ord.lt_le_lt; et.
-  - econs; try apply SIM; et. eapply Ord.lt_le_lt; et.
-  (* - econs; try apply SIM; et. etrans; et. *)
-  - econs; try apply SIM; et. eapply Ord.lt_le_lt; et.
-  - econs; try apply SIM; et. eapply Ord.lt_le_lt; et.
-  (* - econs; try apply SIM; et. etrans; et. *)
-  - econs; try apply SIM; et. eapply Ord.lt_le_lt; et.
-  - econs; try apply SIM; et. eapply Ord.lt_le_lt; et.
-Qed.
-
-
-End TY.
-
-Hint Constructors _simg.
-Hint Unfold simg.
-Hint Resolve simg_mon: paco.
-
-
-
-
-
-
-
-
-
-
-
-
-
-
-
-
-
-Global Program Instance simg_paco_refl r R RR `{Reflexive _ RR} o_src0 o_tgt0
-       (LT: Ord.lt Ord.O o_src0 /\ Ord.lt Ord.O o_tgt0)
-  : Reflexive (paco7 _simg r R R RR o_src0 o_tgt0).
-Next Obligation.
-  revert_until r. pcofix CIH. i. pfold. ides x.
-  - econs; et.
-  - econs 3; et. left. pfold. econs 4; auto.
-    { eapply Ord.S_lt. }
-    right. et.
-  - rewrite <- ! bind_trigger. destruct e.
-    + econs 6; et. i. left. pfold. econs 5; auto.
-      { eapply Ord.S_lt. }
-      esplits. right. et.
-    + econs 7; et. i. left. pfold. econs 8; auto.
-      { eapply Ord.S_lt. }
-      esplits. right. et.
-    + econs; et. i. subst. right. et.
-Qed.
-
-Global Program Instance simg_gpaco_refl r R RR `{Reflexive _ RR} rg o_src0 o_tgt0
-       (LT: Ord.lt Ord.O o_src0 /\ Ord.lt Ord.O o_tgt0)
-  : Reflexive (gpaco7 _simg (cpn7 _simg) r rg R R RR o_src0 o_tgt0).
-Next Obligation.
-  gfinal. right. eapply simg_paco_refl; et.
-Qed.
-
-Global Program Instance simg_refl R RR `{Reflexive _ RR} o_src0 o_tgt0
-       (LT: Ord.lt Ord.O o_src0 /\ Ord.lt Ord.O o_tgt0)
-  : Reflexive (@simg R R RR o_src0 o_tgt0).
-Next Obligation.
-  eapply simg_paco_refl; ss.
-Qed.
-
-
-
-
-
-
-
-
-
-
-
-
-
-
-
-
-
-
-
-
-
-
-Variant ordC (r: forall S0 S1 (SS: S0 -> S1 -> Prop), Ord.t -> Ord.t -> (itree eventE S0) -> (itree eventE S1) -> Prop):
-  forall S0 S1 (SS: S0 -> S1 -> Prop), Ord.t -> Ord.t -> (itree eventE S0) -> (itree eventE S1) -> Prop :=
-| ordC_intro
-    o_src0 o_src1 o_tgt0 o_tgt1 R0 R1 (RR: R0 -> R1 -> Prop) itr_src itr_tgt
-    (ORDSRC: Ord.le o_src0 o_src1)
-    (ORDTGT: Ord.le o_tgt0 o_tgt1)
-    (SIM: r _ _ RR o_src0 o_tgt0 itr_src itr_tgt)
-  :
-    ordC r RR o_src1 o_tgt1 itr_src itr_tgt
-.
-Hint Constructors ordC: core.
-
-Lemma ordC_mon
-      r1 r2
-      (LE: r1 <7= r2)
-  :
-    ordC r1 <7= ordC r2
-.
-Proof. ii. destruct PR; econs; et. Qed.
-Hint Resolve ordC_mon: paco.
-
-Lemma ordC_prespectful: prespectful7 (_simg) ordC.
-Proof.
-  econs; eauto with paco.
-  ii. inv PR. csc.
-  rename x2 into o1. apply GF in SIM. pfold. inv SIM.
-  - econs; eauto.
-  - econs; eauto.
-  - econs; eauto. { eapply Ord.lt_le_lt; et. }
-  - econs; eauto. { eapply Ord.lt_le_lt; et. }
-  - econs; eauto. { eapply Ord.lt_le_lt; et. } des. esplits; et.
-  - econs; eauto. { eapply Ord.lt_le_lt; et. }
-  - econs; eauto. { eapply Ord.lt_le_lt; et. }
-  - econs; eauto. { eapply Ord.lt_le_lt; et. } des. esplits; et.
-Qed.
-
-Lemma ordC_spec: ordC <8= gupaco7 (_simg) (cpn7 _simg).
-Proof. intros. eapply prespect7_uclo; eauto with paco. eapply ordC_prespectful. Qed.
-
-
-
-
-
-
-
-
-
-
-
-Variant bindR (r s: forall S0 S1 (SS: S0 -> S1 -> Prop), Ord.t -> Ord.t -> (itree eventE S0) -> (itree eventE S1) -> Prop):
-  forall S0 S1 (SS: S0 -> S1 -> Prop), Ord.t -> Ord.t -> (itree eventE S0) -> (itree eventE S1) -> Prop :=
-| bindR_intro
-    o_src0 o_src1 o_tgt0 o_tgt1
-
-    R0 R1 RR
-    (i_src: itree eventE R0) (i_tgt: itree eventE R1)
-    (SIM: r _ _ RR o_src0 o_tgt0 i_src i_tgt)
-
-    S0 S1 SS
-    (k_src: ktree eventE R0 S0) (k_tgt: ktree eventE R1 S1)
-    (SIMK: forall vret_src vret_tgt (SIM: RR vret_src vret_tgt), s _ _ SS o_src1 o_tgt1 (k_src vret_src) (k_tgt vret_tgt))
-  :
-    (* bindR r s (Ordinal.add o0 o1) (ITree.bind i_src k_src) (ITree.bind i_tgt k_tgt) *)
-    bindR r s SS (OrdArith.add o_src1 o_src0) (OrdArith.add o_tgt1 o_tgt0) (ITree.bind i_src k_src) (ITree.bind i_tgt k_tgt)
-.
-
-Hint Constructors bindR: core.
-
-Lemma bindR_mon
-      r1 r2 s1 s2
-      (LEr: r1 <7= r2) (LEs: s1 <7= s2)
-  :
-    bindR r1 s1 <7= bindR r2 s2
-.
-Proof. ii. destruct PR; econs; et. Qed.
-
-Definition bindC r := bindR r r.
-Hint Unfold bindC: core.
-
-Lemma bindC_wrespectful: wrespectful7 (_simg) bindC.
-Proof.
-  econstructor; repeat intro.
-  { eapply bindR_mon; eauto. }
-  rename l into llll.
-  eapply bindR_mon in PR; cycle 1.
-  { eapply GF. }
-  { i. eapply PR0. }
-  inv PR. csc. inv SIM.
-  + irw.
-    exploit SIMK; eauto. i.
-    eapply simg_mon_ord.
-    { eapply OrdArith.add_base_l. }
-    { eapply OrdArith.add_base_l. }
-    eapply simg_mon; eauto with paco.
-  + rewrite ! bind_bind. econs; eauto. ii.
-    { econs 2; eauto with paco. econs; eauto with paco. }
-
-  + rewrite ! bind_tau. econs; eauto.
-    { eapply OrdArith.lt_add_r; et. }
-    econs 2; eauto with paco. econs; eauto with paco.
-  + irw. econs; eauto.
-    { eapply OrdArith.lt_add_r; et. }
-    econs 2; eauto with paco. econs; eauto with paco.
-
-  + rewrite ! bind_bind. econs; eauto.
-    { eapply OrdArith.lt_add_r; et. }
-    des. esplits; et. econs 2; eauto with paco. econs; eauto with paco.
-  + rewrite ! bind_bind. econs; eauto.
-    { eapply OrdArith.lt_add_r; et. }
-    des. esplits; et. econs 2; eauto with paco. econs; eauto with paco.
-
-  + rewrite ! bind_bind. econs; eauto.
-    { eapply OrdArith.lt_add_r; et. }
-    des. esplits; et. econs 2; eauto with paco. econs; eauto with paco.
-  + rewrite ! bind_bind. econs; eauto.
-    { eapply OrdArith.lt_add_r; et. }
-    des. esplits; et. econs 2; eauto with paco. econs; eauto with paco.
-Qed.
-
-Lemma bindC_spec: bindC <8= gupaco7 (_simg) (cpn7 (_simg)).
-Proof.
-  intros. eapply wrespect7_uclo; eauto with paco. eapply bindC_wrespectful.
-Qed.
-
-Theorem simg_bind
-        R0 R1 S0 S1
-        RR SS
-        o_src0 o_tgt0 (itr_src: itree eventE R0) (itr_tgt: itree eventE R1)
-        (SIM: simg RR o_src0 o_tgt0 itr_src itr_tgt)
-        o_src1 o_tgt1 (ktr_src: ktree eventE R0 S0) (ktr_tgt: ktree eventE R1 S1)
-        (SIMK: forall vret_src vret_tgt (SIM: RR vret_src vret_tgt), simg SS o_src1 o_tgt1 (ktr_src vret_src) (ktr_tgt vret_tgt))
-  :
-    simg SS (OrdArith.add o_src1 o_src0) (OrdArith.add o_tgt1 o_tgt0)
-         (itr_src >>= ktr_src) (itr_tgt >>= ktr_tgt)
-.
-Proof.
-  ginit.
-  { eapply cpn7_wcompat; eauto with paco. }
-  guclo bindC_spec. econs.
-  - eauto with paco.
-  - ii. exploit SIMK; eauto with paco.
-Qed.
-
-
-
-Lemma step_trigger_choose_iff X k itr e
-      (STEP: ModSemL.step (trigger (Choose X) >>= k) e itr)
-  :
-    exists x,
-      e = None /\ itr = k x.
-Proof.
-  inv STEP.
-  { eapply f_equal with (f:=observe) in H0. ss. }
-  { eapply f_equal with (f:=observe) in H0. ss.
-    unfold trigger in H0. ss. cbn in H0.
-    dependent destruction H0. ired. et.  }
-  { eapply f_equal with (f:=observe) in H0. ss. }
-  { eapply f_equal with (f:=observe) in H0. ss. }
-Qed.
-
-Lemma step_trigger_take_iff X k itr e
-      (STEP: ModSemL.step (trigger (Take X) >>= k) e itr)
-  :
-    exists x,
-      e = None /\ itr = k x.
-Proof.
-  inv STEP.
-  { eapply f_equal with (f:=observe) in H0. ss. }
-  { eapply f_equal with (f:=observe) in H0. ss. }
-  { eapply f_equal with (f:=observe) in H0. ss.
-    unfold trigger in H0. ss. cbn in H0.
-    dependent destruction H0. ired. et.  }
-  { eapply f_equal with (f:=observe) in H0. ss. }
-Qed.
-
-Lemma step_tau_iff itr0 itr1 e
-      (STEP: ModSemL.step (Tau itr0) e itr1)
-  :
-    e = None /\ itr0 = itr1.
-Proof.
-  inv STEP. et.
-Qed.
-
-Lemma step_ret_iff rv itr e
-      (STEP: ModSemL.step (Ret rv) e itr)
-  :
-    False.
-Proof.
-  inv STEP.
-Qed.
-
-Lemma step_trigger_syscall_iff fn args rvs k e itr
-      (STEP: ModSemL.step (trigger (Syscall fn args rvs) >>= k) e itr)
-  :
-    exists rv, itr = k rv /\ e = Some (event_sys fn args rv)
-               /\ <<RV: rvs rv>> /\ <<SYS: syscall_sem (event_sys fn args rv)>>.
-Proof.
-  inv STEP.
-  { eapply f_equal with (f:=observe) in H0. ss. }
-  { eapply f_equal with (f:=observe) in H0. ss. }
-  { eapply f_equal with (f:=observe) in H0. ss. }
-  { eapply f_equal with (f:=observe) in H0. ss.
-    unfold trigger in H0. ss. cbn in H0.
-    dependent destruction H0. ired. et. }
-Qed.
-
-
-Lemma itree_eta_eq E R (itr0 itr1: itree E R)
-    (OBSERVE: observe itr0 = observe itr1)
-  :
-    itr0 = itr1.
-Proof.
-  rewrite (itree_eta_ itr0).
-  rewrite (itree_eta_ itr1).
-  rewrite OBSERVE. auto.
-Qed.
-
-Lemma step_trigger_choose X k x
-  :
-    ModSemL.step (trigger (Choose X) >>= k) None (k x).
-Proof.
-  unfold trigger. ss.
-  match goal with
-  | [ |- ModSemL.step ?itr _ _] =>
-    replace itr with (Subevent.vis (Choose X) k)
-  end; ss.
-  { econs. }
-  { eapply itree_eta_eq. ss. cbv. f_equal.
-    extensionality x0. eapply itree_eta_eq. ss. }
-Qed.
-
-Lemma step_trigger_take X k x
-  :
-    ModSemL.step (trigger (Take X) >>= k) None (k x).
-Proof.
-  unfold trigger. ss.
-  match goal with
-  | [ |- ModSemL.step ?itr _ _] =>
-    replace itr with (Subevent.vis (Take X) k)
-  end; ss.
-  { econs. }
-  { eapply itree_eta_eq. ss. cbv. f_equal.
-    extensionality x0. eapply itree_eta_eq. ss. }
-Qed.
-
-Lemma step_trigger_syscall fn args (rvs: Any.t -> Prop) k rv
-      (RV: rvs rv) (SYS: syscall_sem (event_sys fn args rv))
-  :
-    ModSemL.step (trigger (Syscall fn args rvs) >>= k) (Some (event_sys fn args rv)) (k rv).
-Proof.
-  unfold trigger. ss.
-  match goal with
-  | [ |- ModSemL.step ?itr _ _] =>
-    replace itr with (Subevent.vis (Syscall fn args rvs) k)
-  end; ss.
-  { econs; et. }
-  { eapply itree_eta_eq. ss. cbv. f_equal.
-    extensionality x0. eapply itree_eta_eq. ss. }
-Qed.
-
-Lemma step_tau itr
-  :
-    ModSemL.step (Tau itr) None itr.
-Proof.
-  econs.
-Qed.
-
-Context {CONFS CONFT: EMSConfig}.
-Hypothesis (FINSAME: (@finalize CONFS) = (@finalize CONFT)).
-
-Theorem adequacy_global_itree itr_src itr_tgt
-        (SIM: exists o_src0 o_tgt0, simg eq o_src0 o_tgt0 itr_src itr_tgt)
-  :
-    Beh.of_program (@ModSemL.compile_itree CONFT itr_tgt)
-    <1=
-    Beh.of_program (@ModSemL.compile_itree CONFS itr_src).
-Proof.
-  unfold Beh.of_program. ss.
-  i. destruct SIM as [o_src0 [o_tgt0 SIMG]]. eapply adequacy_aux; et.
-  { eapply Ord.lt_well_founded. }
-  { eapply Ord.lt_well_founded. }
-  instantiate (1:=o_tgt0). instantiate (1:=o_src0). clear x0 PR.
-  generalize itr_tgt at 1 as md_tgt.
-  generalize itr_src at 1 as md_src. i.
-  revert o_src0 o_tgt0 itr_src itr_tgt SIMG. pcofix CIH.
-  i. punfold SIMG. inv SIMG; pfold.
-  { destruct (finalize r_tgt) eqn:T.
-    { eapply sim_fin; ss; cbn; des_ifs; rewrite FINSAME in *; clarify. }
-    { eapply sim_angelic_src.
-      { cbn. des_ifs; rewrite FINSAME in *; clarify. }
-      i. exfalso. inv STEP.
-    }
-  }
-  { eapply sim_vis; ss. i.
-    eapply step_trigger_syscall_iff in STEP. des. clarify.
-    esplits.
-    { eapply step_trigger_syscall; et. }
-    { right. eapply CIH.
-      hexploit SIM; et. i. pclearbot. eapply H. }
-  }
-  { eapply sim_demonic_src; ss.
-    esplits.
-    { eapply step_tau; et. }
-    { et. }
-    { right. eapply CIH. destruct SIM; ss. et. }
-  }
-  { eapply sim_demonic_tgt; ss. i.
-    eapply step_tau_iff in STEP. des. clarify.
-    esplits.
-    { et. }
-    { right. eapply CIH. destruct SIM; ss. et. }
-  }
-  { eapply sim_demonic_src; ss. destruct SIM.
-    esplits.
-    { eapply step_trigger_choose; et. }
-    { et. }
-    { right. eapply CIH. destruct H; ss. apply p. }
-  }
-  { eapply sim_demonic_tgt; ss. i.
-    eapply step_trigger_choose_iff in STEP. des. clarify.
-    hexploit (SIM x); et. i. des.
-    esplits.
-    { et. }
-    { right. eapply CIH. destruct H; ss. et. }
-  }
-  { eapply sim_angelic_src; ss. i.
-    eapply step_trigger_take_iff in STEP. des. clarify.
-    hexploit (SIM x); et. i. des.
-    esplits.
-    { et. }
-    { right. eapply CIH. destruct H; ss. et. }
-  }
-  { eapply sim_angelic_tgt; ss. destruct SIM.
-    esplits.
-    { eapply step_trigger_take; et. }
-    { et. }
-    { right. eapply CIH. destruct H; ss. apply p. }
-  }
-Qed.
-
-
-Variable md_src md_tgt: ModL.t.
-Let ms_src: ModSemL.t := md_src.(ModL.enclose).
-Let ms_tgt: ModSemL.t := md_tgt.(ModL.enclose).
-
-Section ADEQUACY.
-Hypothesis (SIM: exists o_src0 o_tgt0, simg eq o_src0 o_tgt0 (@ModSemL.initial_itr ms_src CONFS (Some (ModL.wf md_src))) (@ModSemL.initial_itr ms_tgt CONFT (Some (ModL.wf md_tgt)))).
-
-
-Theorem adequacy_global: Beh.of_program (@ModL.compile _ CONFT md_tgt) <1= Beh.of_program (@ModL.compile _ CONFS md_src).
-Proof.
-  eapply adequacy_global_itree. eapply SIM.
-Qed.
-End ADEQUACY.
-End SIM.
-
-Hint Constructors _simg.
-Hint Unfold simg.
-Hint Resolve simg_mon: paco.
-Hint Constructors ordC: core.
-Hint Resolve ordC_mon: paco.
-Hint Constructors bindR: core.
-Hint Unfold bindC: core.
-
-
-Inductive _simg_safe (simg: forall R0 R1 (RR: R0 -> R1 -> Prop), Ord.t -> Ord.t -> (itree eventE R0) -> (itree eventE R1) -> Prop)
-          {R0 R1} (RR: R0 -> R1 -> Prop) (i_src0 i_tgt0: Ord.t): (itree eventE R0) -> (itree eventE R1) -> Prop :=
-| simg_safe_ret
-    r_src r_tgt
-    (SIM: RR r_src r_tgt)
-  :
-    _simg_safe simg RR i_src0 i_tgt0 (Ret r_src) (Ret r_tgt)
-| simg_safe_syscall
-    i_src1 i_tgt1 ktr_src0 ktr_tgt0 fn varg rvs
-    (SIM: forall x_src x_tgt (EQ: x_src = x_tgt), simg _ _ RR i_src1 i_tgt1 (ktr_src0 x_src) (ktr_tgt0 x_tgt))
-  :
-    _simg_safe simg RR i_src0 i_tgt0 (trigger (Syscall fn varg rvs) >>= ktr_src0) (trigger (Syscall fn varg rvs) >>= ktr_tgt0)
-
-
-| simg_safe_tauL
-    i_src1 i_tgt1 itr_src0 itr_tgt0
-    (TAUL: True)
-    (ORD: Ord.lt i_tgt1 i_tgt0)
-    (SIM: simg _ _ RR i_src1 i_tgt1 itr_src0 itr_tgt0)
-  :
-    _simg_safe simg RR i_src0 i_tgt0 (tau;; itr_src0) (itr_tgt0)
-| simg_safe_tauR
-    i_src1 i_tgt1 itr_src0 itr_tgt0
-    (TAUR: True)
-    (ORD: Ord.lt i_src1 i_src0)
-    (SIM: simg _ _ RR i_src1 i_tgt1 itr_src0 itr_tgt0)
-  :
-    _simg_safe simg RR i_src0 i_tgt0 (itr_src0) (tau;; itr_tgt0)
-
-
-| simg_safe_chooseR
-    i_src1 i_tgt1 X itr_src0 ktr_tgt0
-    (CHOOSER: True)
-    (ORD: Ord.lt i_src1 i_src0)
-    (SIM: forall x, simg _ _ RR i_src1 i_tgt1 itr_src0 (ktr_tgt0 x))
-  :
-    _simg_safe simg RR i_src0 i_tgt0 (itr_src0) (trigger (Choose X) >>= ktr_tgt0)
-
-
-| simg_safe_takeL
-    i_src1 i_tgt1 X ktr_src0 itr_tgt0
-    (TAKEL: True)
-    (ORD: Ord.lt i_tgt1 i_tgt0)
-    (SIM: forall x, simg _ _ RR i_src1 i_tgt1 (ktr_src0 x) itr_tgt0)
-  :
-    _simg_safe simg RR i_src0 i_tgt0 (trigger (Take X) >>= ktr_src0) (itr_tgt0)
-.
-
-Lemma simg_safe_spec:
-  _simg_safe <8= _simg.
-Proof. i. inv PR; try by (econs; eauto). Qed.
